WhileD/WhileDCompleteness.v
@@ -6,7 +6,6 @@ Require Import Coq.ZArith.ZArith.
 Require Import Coq.micromega.Psatz.
 Require Import SetsClass.SetsClass. Import SetsNotation.
 Require Import PV.Syntax.
-Require Import PV.DenotationalSemantics.
 Require Import PV.WhileDDenotations.
 Require Import PV.HoareLogic.
 Local Open Scope string.
@@ -16,11 +15,14 @@ Local Open Scope sets.
 Arguments Rels.concat: simpl never.
 Arguments Sets.indexed_union: simpl never.
 
-Import  Lang_WhileD
-        DntSem_WhileD.
+Import Lang_While.
+Import Lang_WhileD.
+Import DntSem_WhileD.
+Import HoareWhileD.
+Import HoareWhileD_Admissible.
 
 Definition wp (c:com) (Q:assertion) : assertion :=
-  fun s => forall s', eval_com c s s' -> Q s'.
+  fun s => forall s', (eval_com c).(nrm) s s' -> Q s'.
 
 Hint Unfold wp : core.
 
@@ -50,18 +52,19 @@ Qed.
 
 Lemma wp_seq : forall P Q c1 c2,
     provable {{P}} c1 {{(wp c2 Q)}} -> 
-    provable {{(wp c2 Q)}} c2 {{Q}} -> provable {{P}} [[c1; c2]] {{Q}}.
+    provable {{(wp c2 Q)}} c2 {{Q}} -> provable {{P}} (c1; c2) {{Q}}.
 Proof.
   intros.
   eapply hoare_seq; [apply H|apply H0].
 Qed.
 
 Lemma wp_invariant : forall b c Q,
-    valid {{ (wp (CWhile b c) Q) && [[ b ]] }} c {{ wp (CWhile b c) Q }}.
+    valid {{ (wp (CWhile b c) Q) && (eb2assn b) }} c {{ wp (CWhile b c) Q }}.
 Proof.
   unfold valid.
   unfold wp.
-  assn_unfold.
+  unfold andp.
+  simpl.
   intros.
   destruct H.
   specialize (H s').
@@ -73,8 +76,9 @@ Proof.
   intros.
   destruct H1.
   exists (S x).
-  simpl.
+  simpl.  
   unfold_RELS_tac.
+  left.
   exists s1.
   split.
   + unfold test_true.
@@ -85,15 +89,20 @@ Proof.
   + exists s2.
     tauto.
 Qed.
+(* 
+Lemma concat_empty: 
+  forall X,
+  Rels.concat X Sets.empty = Sets.empty. *)
 
-Theorem hoare_complet: forall P Q c,
+Theorem hoare_complete: forall P Q c,
    valid {{ P }} c {{ Q }} -> provable {{ P }} c {{ Q }}.
 Proof.
   unfold valid.
   intros; revert P Q H.
   induction c; intros P Q HT. 
   + assert (P |-- Q).
-    - assn_unfold.
+    - intros.
+      unfold derives.
       intros.
       specialize (HT s s).
       apply HT; auto.
@@ -103,28 +112,9 @@ Proof.
       reflexivity.
     - eapply hoare_conseq_post; [|apply H].
       apply (hoare_skip P).
-  + pose proof (hoare_asgn_fwd P x e).
-    apply (hoare_conseq_post _ _ _ _ H).
-    assn_unfold; simpl.
-    unfold const_sem.
-    unfold_substs.
-    unfold var_sem.
-    unfold ei2exprZ.
-    unfold exp.
-    unfold exprZ_eq.
-    intros.
-    destruct H0 as [n [? ?] ].
-    pose proof (HT (state_subst s x n) s).
-    apply H2; auto.
-    unfold eval_com.
-    unfold asgn_sem.
-    split; auto.
-    intros.
-    unfold state_subst.
-    destruct (x =? Y)%string eqn : I; auto.
-    apply String.eqb_eq in I.
-    rewrite I in H3; contradiction.
-  + apply (hoare_seq P (fun s => exists x: state, P x /\ eval_com c1 x s) Q).
+  + admit.
+  + admit.
+  + apply (hoare_seq P (fun s => exists x: state, P x /\ (eval_com c1).(nrm) x s) Q).
     - apply IHc1.
       intros.
       exists s1.
@@ -139,7 +129,7 @@ Proof.
       unfold_RELS_tac.
       exists s1; tauto.
   + apply hoare_if.
-    - specialize (IHc1 Assn(P && [[e]]) Q).
+    - specialize (IHc1 Assn(P && (eb2assn e)) Q).
       apply IHc1.
       intros.
       specialize (HT s1 s2); apply HT.
@@ -153,7 +143,7 @@ Proof.
         split; auto.
         split; auto.
         revert H; assn_unfold; tauto.
-    - specialize (IHc2 Assn(P && [[!e]]) Q).
+    - specialize (IHc2 Assn(P && (eb2assn_not e)) Q).
       apply IHc2.
       intros.
       specialize (HT s1 s2); apply HT.
@@ -172,9 +162,18 @@ Proof.
         unfold not_sem.
         intros.
         unfold negb in H; destruct H.
-        destruct (eval_expr_bool e s1); auto.
+        unfold eb2assn_not in H1.
+        destruct H1.
+        destruct H1.
+        assert(x = Integers.Int64.repr 0).
+        ++  rewrite <- H2.
+            pose proof Integers.Int64.repr_signed x.
+            rewrite H3.
+            reflexivity.
+        ++  subst x.
+            tauto. 
   + pose proof wp_invariant e c Q.
-    specialize (IHc  Assn((wp (CWhile e c) Q) && [[e]])  (wp (CWhile e c) Q)).
+    specialize (IHc  Assn((wp (CWhile e c) Q) && (eb2assn e))  (wp (CWhile e c) Q)).
     unfold valid in H.
     apply IHc in H.
     apply hoare_while in H.
@@ -196,13 +195,26 @@ Proof.
       unfold while_sem.
       unfold_RELS_tac.
       unfold eb2assn.
+      unfold eb2assn_not.
       simpl.
       unfold not_sem.
       unfold negb.
       intros.
-      exists O. simpl.
+      exists (S O).
+      unfold iter_nrm_lt_n.
+      unfold Sets.union.
+      simpl.
+      right.
       unfold test_false.
       unfold_RELS_tac.
       split; [|tauto].
-      destruct (eval_expr_bool e s); auto.
+      destruct H1.
+      destruct H1.
+      assert(x = Integers.Int64.repr 0).
+      ++  rewrite <- H2.
+          pose proof Integers.Int64.repr_signed x.
+          rewrite H3.
+          reflexivity.
+      ++  subst x.
+          tauto.
 Qed.
